Finish proof. Need to prove one last lemma

CPL/b_sequent_calculus.v
@@ -11,17 +11,22 @@ Notation "Γ ⇒ Δ" := (Arrow Γ Δ) (at level 80): My_scope.
 (* To fix, turn inductive type wrt Seq *)
 
 Inductive DerSeq_P : Seq -> Prop :=
-  | SId   : forall A Γ Δ      , In A Γ                      -> In A Δ                     -> DerSeq_P (Γ ⇒ Δ)
-  | SBotL : forall A Γ1 Γ2 Δ1 Δ2  , DerSeq_P (Γ1++Γ2 ⇒ Δ1++A::Δ2) -> DerSeq_P (Γ1++¬A::Γ2 ⇒ Δ1++Δ2)
-  | SBotR : forall A Γ1 Γ2 Δ1 Δ2  , DerSeq_P (Γ1++A::Γ2 ⇒ Δ1++Δ2) -> DerSeq_P (Γ1++Γ2 ⇒ Δ1++¬A::Δ2)
-  | SRBotL : forall A Γ1 Γ2 Δ1 Δ2  , DerSeq_P (Γ1++¬A::Γ2 ⇒ Δ1++Δ2) -> DerSeq_P (Γ1++Γ2 ⇒ Δ1++A::Δ2)
-  | SRBotR : forall A Γ1 Γ2 Δ1 Δ2  , DerSeq_P (Γ1++Γ2 ⇒ Δ1++¬A::Δ2) -> DerSeq_P (Γ1++A::Γ2 ⇒ Δ1++Δ2)
-  | SAndL : forall A B Γ1 Γ2 Δ, DerSeq_P (Γ1++A::B::Γ2 ⇒ Δ)                               -> DerSeq_P (Γ1++A∧B::Γ2 ⇒ Δ)
-  | SAndR : forall A B Γ Δ1 Δ2, DerSeq_P (Γ ⇒ Δ1++A::Δ2)    -> DerSeq_P (Γ ⇒ Δ1++B::Δ2)   -> DerSeq_P (Γ ⇒ Δ1++A∧B::Δ2)
-  (*| SOrL  : forall A B Γ1 Γ2 Δ, DerSeq_P (Γ1++A::Γ2 ⇒ Δ)    -> DerSeq_P (Γ1++B::Γ2 ⇒ Δ)   -> DerSeq_P (Γ1++A∨B::Γ2 ⇒ Δ)
-  | SOrR  : forall A B Γ Δ1 Δ2, DerSeq_P (Γ ⇒ Δ1++A::B::Δ2)                               -> DerSeq_P (Γ ⇒ Δ1++A∨B::Δ2)
-  | SImpL : forall A B Γ1 Γ2 Δ, DerSeq_P (Γ1++B::Γ2 ⇒ Δ)    -> DerSeq_P (Γ1++Γ2 ⇒ A::Δ)   -> DerSeq_P (Γ1++A→B::Γ2 ⇒ Δ)
-  | SImpR : forall Γ Δ1 Δ2 A B, DerSeq_P (A::Γ ⇒ Δ1++B::Δ2)                               -> DerSeq_P (Γ ⇒ Δ1++A→B::Δ2)
-*).
+  | SId   : forall A Γ Δ          , In A Γ                           -> In A Δ                        -> DerSeq_P (Γ ⇒ Δ)
+  | SBot  : forall Γ Δ            , In ⊥ Γ                                                            -> DerSeq_P (Γ ⇒ Δ)
+  | SAndL : forall A B Γ1 Γ2 Δ    , DerSeq_P (Γ1++A::B::Γ2 ⇒ Δ)                                       -> DerSeq_P (Γ1++A∧B::Γ2 ⇒ Δ)
+  | SAndR : forall A B Γ Δ1 Δ2    , DerSeq_P (Γ ⇒ Δ1++A::Δ2)         -> DerSeq_P (Γ ⇒ Δ1++B::Δ2)      -> DerSeq_P (Γ ⇒ Δ1++A∧B::Δ2)
+  | SOrL  : forall A B Γ1 Γ2 Δ    , DerSeq_P (Γ1++A::Γ2 ⇒ Δ)         -> DerSeq_P (Γ1++B::Γ2 ⇒ Δ)      -> DerSeq_P (Γ1++A∨B::Γ2 ⇒ Δ)
+  | SOrR  : forall A B Γ Δ1 Δ2    , DerSeq_P (Γ ⇒ Δ1++A::B::Δ2)                                       -> DerSeq_P (Γ ⇒ Δ1++A∨B::Δ2)
+  | SImpL : forall A B Γ1 Γ2 Δ1 Δ2, DerSeq_P (Γ1++B::Γ2 ⇒ Δ1++Δ2)    -> DerSeq_P (Γ1++Γ2 ⇒ Δ1++A::Δ2) -> DerSeq_P (Γ1++A→B::Γ2 ⇒ Δ1++Δ2)
+  | SImpR : forall A B Γ1 Γ2 Δ1 Δ2, DerSeq_P (Γ1++A::Γ2 ⇒ Δ1++B::Δ2)                                  -> DerSeq_P (Γ1++Γ2 ⇒ Δ1++A→B::Δ2)
+  .
+
+Check DerSeq_P.
+
+Theorem test : forall A, DerSeq_P (A::nil ⇒ A::nil).
+Proof.
+  intros.
+  apply (SId A). intuition. intuition.
+Qed.
 
 End sequent_calculus_mod.
